Hoare Simulation iProp style

proofmode/HSim.v
@@ -123,6 +123,7 @@ Section SIM.
       (MEASURE: o = ord_top)
       (NPURE: fsp.(measure) x = ord_top)
       (POST: forall ctx1 w1 st_src1 st_tgt1 ret_src ret_tgt
+                    (LE: le w0 w1)
                     (ACC: current_iProp ctx1 (FR ** I w1 st_src1 st_tgt1 ** fsp.(postcond) (Some mn) x ret_src ret_tgt)),
           hsim _ _ Q ctx1 None true true (st_src1, ktr_src ret_src) (st_tgt1, ktr_tgt ret_tgt))
     :
@@ -146,6 +147,7 @@ Section SIM.
       (POST: exists fuel1,
           (<<FUEL: Ord.lt fuel1 fuel0>>) /\
           (<<SIM: forall ctx1 w1 st_src1 st_tgt1 ret_src ret_tgt
+                         (LE: le w0 w1)
                          (ACC: current_iProp ctx1 (FR ** I w1 st_src1 st_tgt1 ** fsp.(postcond) (Some mn) x ret_src ret_tgt)),
               hsim _ _ Q ctx1 (Some fuel1) true true (st_src1, itr_src) (st_tgt1, ktr_tgt ret_tgt)>>))
     :
@@ -255,6 +257,7 @@ Section SIM.
             (MEASURE: o = ord_top)
             (NPURE: fsp.(measure) x = ord_top)
             (POST: forall ctx1 w1 st_src1 st_tgt1 ret_src ret_tgt
+                          (LE: le w0 w1)
                           (ACC: current_iProp ctx1 (FR ** I w1 st_src1 st_tgt1 ** fsp.(postcond) (Some mn) x ret_src ret_tgt)),
                 hsim _ _ Q ctx1 None true true (st_src1, ktr_src ret_src) (st_tgt1, ktr_tgt ret_tgt)),
             P fuel f_src f_tgt (st_src0, trigger (Call fn arg_src) >>= ktr_src) (st_tgt0, trigger (Call fn arg_tgt) >>= ktr_tgt))
@@ -277,6 +280,7 @@ Section SIM.
             (POST: exists fuel1,
                 (<<FUEL: Ord.lt fuel1 fuel0>>) /\
                 (<<SIM: forall ctx1 w1 st_src1 st_tgt1 ret_src ret_tgt
+                               (LE: le w0 w1)
                                (ACC: current_iProp ctx1 (FR ** I w1 st_src1 st_tgt1 ** fsp.(postcond) (Some mn) x ret_src ret_tgt)),
                     hsim _ _ Q ctx1 (Some fuel1) true true (st_src1, itr_src) (st_tgt1, ktr_tgt ret_tgt)>>)),
             P (Some fuel0) f_src f_tgt (st_src0, itr_src) (st_tgt0, trigger (Call fn arg_tgt) >>= ktr_tgt))
@@ -423,6 +427,7 @@ Section SIM.
             (MEASURE: o = ord_top)
             (NPURE: fsp.(measure) x = ord_top)
             (POST: forall ctx1 w1 st_src1 st_tgt1 ret_src ret_tgt
+                          (LE: le w0 w1)
                           (ACC: current_iProp ctx1 (FR ** I w1 st_src1 st_tgt1 ** fsp.(postcond) (Some mn) x ret_src ret_tgt)),
                 hsim Q ctx1 None true true (st_src1, ktr_src ret_src) (st_tgt1, ktr_tgt ret_tgt)),
             P fuel f_src f_tgt (st_src0, trigger (Call fn arg_src) >>= ktr_src) (st_tgt0, trigger (Call fn arg_tgt) >>= ktr_tgt))
@@ -445,6 +450,7 @@ Section SIM.
             (POST: exists fuel1,
                 (<<FUEL: Ord.lt fuel1 fuel0>>) /\
                 (<<SIM: forall ctx1 w1 st_src1 st_tgt1 ret_src ret_tgt
+                               (LE: le w0 w1)
                                (ACC: current_iProp ctx1 (FR ** I w1 st_src1 st_tgt1 ** fsp.(postcond) (Some mn) x ret_src ret_tgt)),
                     hsim Q ctx1 (Some fuel1) true true (st_src1, itr_src) (st_tgt1, ktr_tgt ret_tgt)>>)),
             P (Some fuel0) f_src f_tgt (st_src0, itr_src) (st_tgt0, trigger (Call fn arg_tgt) >>= ktr_tgt))
@@ -593,7 +599,7 @@ Section SIM.
         { iModIntro. iSplitL "A1"; eauto. iApply "A". }
         { rewrite MEASURE in *. splits; ss. unfold ord_lt. des_ifs. }
         { steps. gbase. hexploit CIH.
-          { eapply POST. eapply current_iProp_entail; [eauto|].
+          { eapply POST; [eauto|]. eapply current_iProp_entail; [eauto|].
             start_ipm_proof. iSplitR "POST".
             { iSplitL "H"; eauto. }
             { iApply "POST". }
@@ -605,7 +611,7 @@ Section SIM.
         { iModIntro. iSplitL "A1"; eauto. iApply "A". }
         { rewrite MEASURE in *. splits; ss. unfold ord_lt. des_ifs. }
         { steps. gbase. hexploit CIH.
-          { eapply POST. eapply current_iProp_entail; [eauto|].
+          { eapply POST; [eauto|]. eapply current_iProp_entail; [eauto|].
             start_ipm_proof. iSplitR "POST".
             { iSplitL "H"; eauto. }
             { iApply "POST". }
@@ -618,8 +624,11 @@ Section SIM.
       { astop. steps. exploit IHSIM; eauto. i. destruct fuel1; ss.
         { astart t0.
           match goal with
-          | x0: ?P1 (_, ?itr0) _ |- ?P0 (_, ?itr1) _ =>
-            replace itr1 with itr0
+          | |- ?P0 (_, ?itr1) _ =>
+            match (type of x0) with
+            | ?P1 (_, ?itr0) _ =>
+              replace itr1 with itr0
+            end
           end; auto.
           grind. destruct x1, x2. destruct u, u0. grind.
         }
@@ -628,8 +637,11 @@ Section SIM.
       { exploit IHSIM; eauto. i. destruct fuel1; ss.
         { astart t.
           match goal with
-          | x0: ?P1 (_, ?itr0) _ |- ?P0 (_, ?itr1) _ =>
-            replace itr1 with itr0
+          | |- ?P0 (_, ?itr1) _ =>
+            match (type of x0) with
+            | ?P1 (_, ?itr0) _ =>
+              replace itr1 with itr0
+            end
           end; auto.
           grind. destruct x1, x2. destruct u, u0. grind.
         }
@@ -647,7 +659,7 @@ Section SIM.
       { iModIntro. iSplitL "A1"; eauto. iApply "A". }
       { splits; ss. }
       { steps. gbase. hexploit CIH.
-        { eapply SIM. eapply current_iProp_entail; [eauto|].
+        { eapply SIM; [eauto|]. eapply current_iProp_entail; [eauto|].
           start_ipm_proof. iSplitR "POST".
           { iSplitL "H"; eauto. }
           { iApply "POST". }
@@ -686,6 +698,149 @@ Section SIM.
     { steps. exploit IHSIM; eauto. }
     { deflag. gbase. eapply CIH; eauto. }
   Qed.
+
+  Lemma hsim_adequacy:
+    forall
+      f_src f_tgt st_src st_tgt (itr_src: itree (hAPCE +' Es) Any.t) itr_tgt mr_src ctx X (x: X) Q mn_caller w0
+      (SIM: hsim (fun st_src st_tgt ret_src ret_tgt =>
+                    (∃ w1, ⌜le w0 w1⌝ ** I w1 st_src st_tgt) ** (Q mn_caller x ret_src ret_tgt: iProp)) ctx None f_src f_tgt (st_src, itr_src) (st_tgt, itr_tgt)),
+      paco8 (_sim_itree (mk_wf I) le) bot8 Any.t Any.t (lift_rel (mk_wf I) le w0 (@eq Any.t))
+            f_src f_tgt w0
+            (Any.pair st_src mr_src,
+             (interp_hCallE_tgt mn stb o (interp_hEs_tgt itr_src) ctx) >>= (HoareFunRet Q mn_caller x))
+            (st_tgt, itr_tgt).
+  Proof.
+    i. hexploit hsim_adequacy_aux; eauto.
+  Qed.
+
+  (* Definition mylift_pure (fuel: option Ord.t) (mn_caller: option mname) X (x: X) *)
+  (*            ctx *)
+  (*            (Q: option mname -> X -> Any.t -> Any.t -> iProp)  *)
+  (*   : itree Es Any.t := *)
+  (*   match fuel with *)
+  (*   | None => *)
+  (*     (interp_hCallE_tgt mn stb o (trigger (Choose _)) ctx) >>= (HoareFunRet Q mn_caller x)      *)
+  (*   | Some fuel => *)
+  (*     (interp_hCallE_tgt mn stb o (_ <- (_APC fuel);; trigger (Choose _)) ctx) >>= (HoareFunRet Q mn_caller x) *)
+  (*   end. *)
+
+  (* Lemma hsim_adequacy_aux_pure: *)
+  (*   forall *)
+  (*     f_src f_tgt st_src st_tgt itr_tgt mr_src ctx X (x: X) Q mn_caller fuel w0 *)
+  (*     (SIM: hsim (fun st_src st_tgt ret_src ret_tgt => *)
+  (*                   (∃ w1, ⌜le w0 w1⌝ ** I w1 st_src st_tgt) ** (Q mn_caller x ret_src ret_tgt: iProp)) ctx fuel f_src f_tgt (st_src, trigger (Choose _)) (st_tgt, itr_tgt)), *)
+  (*     paco8 (_sim_itree (mk_wf I) le) bot8 Any.t Any.t (lift_rel (mk_wf I) le w0 (@eq Any.t)) *)
+  (*           f_src f_tgt w0 *)
+  (*           (Any.pair st_src mr_src, *)
+  (*            mylift_pure fuel mn_caller x ctx Q) *)
+  (*           (st_tgt, itr_tgt). *)
+  (* Proof. *)
+  (*   ginit. gcofix CIH. i. *)
+  (*   remember (st_src, itr_src). remember (st_tgt, itr_tgt). *)
+  (*   revert st_src st_tgt itr_src itr_tgt Heqp Heqp0 CIH. *)
+  (*   induction SIM using hsim_ind; i; clarify. *)
+  (*   { eapply current_iPropL_convert in RET. mDesAll. destruct fuel; steps. *)
+  (*     { astop. steps. hret _; eauto. iModIntro. iSplitL "A1"; auto. } *)
+  (*     { hret _; eauto. iModIntro. iSplitL "A1"; auto. } *)
+  (*   } *)
+  (*   { eapply current_iPropL_convert in PRE. mDesAll. destruct fuel; steps. *)
+  (*     { astop. steps. rewrite SPEC. steps. destruct fsp. ss. hcall _ _ with "A A1". *)
+  (*       { iModIntro. iSplitL "A1"; eauto. iApply "A". } *)
+  (*       { rewrite MEASURE in *. splits; ss. unfold ord_lt. des_ifs. } *)
+  (*       { steps. gbase. hexploit CIH. *)
+  (*         { eapply POST. eapply current_iProp_entail; [eauto|]. *)
+  (*           start_ipm_proof. iSplitR "POST". *)
+  (*           { iSplitL "H"; eauto. } *)
+  (*           { iApply "POST". } *)
+  (*         } *)
+  (*         i. ss. eauto. *)
+  (*       } *)
+  (*     } *)
+  (*     { rewrite SPEC. steps. destruct fsp. ss. hcall _ _ with "A A1". *)
+  (*       { iModIntro. iSplitL "A1"; eauto. iApply "A". } *)
+  (*       { rewrite MEASURE in *. splits; ss. unfold ord_lt. des_ifs. } *)
+  (*       { steps. gbase. hexploit CIH. *)
+  (*         { eapply POST. eapply current_iProp_entail; [eauto|]. *)
+  (*           start_ipm_proof. iSplitR "POST". *)
+  (*           { iSplitL "H"; eauto. } *)
+  (*           { iApply "POST". } *)
+  (*         } *)
+  (*         i. ss. eauto. *)
+  (*       } *)
+  (*     } *)
+  (*   } *)
+  (*   { destruct fuel; steps. *)
+  (*     { astop. steps. exploit IHSIM; eauto. i. destruct fuel1; ss. *)
+  (*       { astart t0. *)
+  (*         match goal with *)
+  (*         | x0: ?P1 (_, ?itr0) _ |- ?P0 (_, ?itr1) _ => *)
+  (*           replace itr1 with itr0 *)
+  (*         end; auto. *)
+  (*         grind. destruct x1, x2. destruct u, u0. grind. *)
+  (*       } *)
+  (*       { astop. steps. } *)
+  (*     } *)
+  (*     { exploit IHSIM; eauto. i. destruct fuel1; ss. *)
+  (*       { astart t. *)
+  (*         match goal with *)
+  (*         | x0: ?P1 (_, ?itr0) _ |- ?P0 (_, ?itr1) _ => *)
+  (*           replace itr1 with itr0 *)
+  (*         end; auto. *)
+  (*         grind. destruct x1, x2. destruct u, u0. grind. *)
+  (*       } *)
+  (*       { astop. steps. } *)
+  (*     } *)
+  (*   } *)
+  (*   { des. steps. rewrite unfold_APC. steps. *)
+  (*     force_l. exists false. steps. *)
+  (*     force_l. exists fuel1. steps. *)
+  (*     force_l; [eauto|..]. steps. *)
+  (*     force_l. exists (fn, arg_src). steps. *)
+  (*     rewrite SPEC. steps. *)
+  (*     eapply current_iPropL_convert in PRE. mDesAll. *)
+  (*     destruct fsp. ss. hcall _ _ with "A A1". *)
+  (*     { iModIntro. iSplitL "A1"; eauto. iApply "A". } *)
+  (*     { splits; ss. } *)
+  (*     { steps. gbase. hexploit CIH. *)
+  (*       { eapply SIM. eapply current_iProp_entail; [eauto|]. *)
+  (*         start_ipm_proof. iSplitR "POST". *)
+  (*         { iSplitL "H"; eauto. } *)
+  (*         { iApply "POST". } *)
+  (*       } *)
+  (*       i. ss. eauto. *)
+  (*     } *)
+  (*   } *)
+  (*   { destruct fuel; steps. *)
+  (*     { astop. steps. gbase. hexploit CIH; eauto. } *)
+  (*     { gbase. hexploit CIH; eauto. } *)
+  (*   } *)
+  (*   { destruct fuel; steps. *)
+  (*     { astop. steps. exploit IHSIM; eauto. } *)
+  (*     { exploit IHSIM; eauto. } *)
+  (*   } *)
+  (*   { steps. exploit IHSIM; eauto. } *)
+  (*   { des. exploit IH; eauto. i. destruct fuel; steps. *)
+  (*     { astop. steps. force_l. eexists. steps. eauto. } *)
+  (*     { force_l. eexists. steps. eauto. } *)
+  (*   } *)
+  (*   { steps. exploit SIM; eauto. i. des. eauto. } *)
+  (*   { destruct fuel; steps. *)
+  (*     { astop. steps. exploit SIM; eauto. i. des. eauto. } *)
+  (*     { exploit SIM; eauto. i. des. eauto. } *)
+  (*   } *)
+  (*   { des. exploit IH; eauto. i. force_r. eexists. eauto. } *)
+  (*   { destruct fuel; steps. *)
+  (*     { astop. steps. exploit IHSIM; eauto. } *)
+  (*     { exploit IHSIM; eauto. } *)
+  (*   } *)
+  (*   { steps. exploit IHSIM; eauto. } *)
+  (*   { destruct fuel; steps. *)
+  (*     { astop. steps. exploit IHSIM; eauto. } *)
+  (*     { exploit IHSIM; eauto. } *)
+  (*   } *)
+  (*   { steps. exploit IHSIM; eauto. } *)
+  (*   { deflag. gbase. eapply CIH; eauto. } *)
+  (* Qed. *)
 
   Lemma hsim_progress_flag R_src R_tgt r g Q ctx fuel st_src st_tgt
         (SIM: gpaco9 _hsim (cpn9 _hsim) g g R_src R_tgt Q ctx fuel false false st_src st_tgt)
@@ -868,6 +1023,7 @@ Section SIM.
       (MEASURE: o = ord_top)
       (NPURE: fsp.(measure) x = ord_top)
       (POST: forall ctx1 w1 st_src1 st_tgt1 ret_src ret_tgt
+                    (LE: le w0 w1)
                     (ACC: current_iProp ctx1 (FR ** I w1 st_src1 st_tgt1 ** fsp.(postcond) (Some mn) x ret_src ret_tgt)),
           g _ _ Q ctx1 None true true (st_src1, ktr_src ret_src) (st_tgt1, ktr_tgt ret_tgt))
     :
@@ -891,6 +1047,7 @@ Section SIM.
       (POST: exists fuel1,
           (<<FUEL: Ord.lt fuel1 fuel0>>) /\
           (<<SIM: forall ctx1 w1 st_src1 st_tgt1 ret_src ret_tgt
+                         (LE: le w0 w1)
                          (ACC: current_iProp ctx1 (FR ** I w1 st_src1 st_tgt1 ** fsp.(postcond) (Some mn) x ret_src ret_tgt)),
               g _ _ Q ctx1 (Some fuel1) true true (st_src1, itr_src) (st_tgt1, ktr_tgt ret_tgt)>>))
     :
@@ -1399,5 +1556,134 @@ Section SIM.
         eapply URA.wf_mon. instantiate (1:=ctx0). r_wf H0.
       }
     }
+  Qed.
+
+  Definition back
+             (r g: forall R_src R_tgt
+                          (Q: Any.t -> Any.t -> R_src -> R_tgt -> iProp)
+                          (ctx: Σ),
+                 option Ord.t -> bool -> bool -> Any.t * itree hEs R_src -> Any.t * itree Es R_tgt -> Prop)
+             {R_src R_tgt}
+             (Q: Any.t -> Any.t -> R_src -> R_tgt -> iProp)
+             (fuel: option Ord.t)
+             (f_src f_tgt: bool)
+             (st_src: Any.t * itree hEs R_src)
+             (st_tgt: Any.t * itree Es R_tgt): iProp :=
+    fun res =>
+      forall ctx (WF: URA.wf (res ⋅ ctx)),
+        gpaco9 (_hsim) (cpn9 _hsim) r g _ _ Q ctx fuel f_src f_tgt st_src st_tgt.
+
+  Lemma back_mono R_src R_tgt
+        (Q0 Q1: Any.t -> Any.t -> R_src -> R_tgt -> iProp)
+        r g fuel f_src f_tgt st_src itr_src st_tgt itr_tgt
+        (MONO: forall st_src st_tgt ret_src ret_tgt,
+            (bi_entails (Q0 st_src st_tgt ret_src ret_tgt) (#=> Q1 st_src st_tgt ret_src ret_tgt)))
+    :
+      bi_entails
+        (back r g Q0 fuel f_src f_tgt (st_src, itr_src) (st_tgt, itr_tgt))
+        (back r g Q1 fuel f_src f_tgt (st_src, itr_src) (st_tgt, itr_tgt)).
+  Proof.
+    red. unfold Entails. autorewrite with iprop.
+    unfold back in *. i. hexploit H; eauto. i.
+    guclo hmonoC_spec. econs; eauto.
+  Qed.
+
+  Lemma back_wand R_src R_tgt
+        (Q0 Q1: Any.t -> Any.t -> R_src -> R_tgt -> iProp)
+        r g fuel f_src f_tgt st_src itr_src st_tgt itr_tgt
+    :
+      bi_entails
+        ((∀ st_src st_tgt ret_src ret_tgt,
+             ((Q0 st_src st_tgt ret_src ret_tgt) -∗ (#=> Q1 st_src st_tgt ret_src ret_tgt))) ** (back r g Q0 fuel f_src f_tgt (st_src, itr_src) (st_tgt, itr_tgt)))
+        (back r g Q1 fuel f_src f_tgt (st_src, itr_src) (st_tgt, itr_tgt)).
+  Proof.
+    red. unfold Entails. autorewrite with iprop.
+    unfold back in *. i.
+    red in H. unfold Sepconj in H. autorewrite with iprop in H.
+    des. clarify. eapply from_semantic in H0. hexploit (H1 (ctx ⋅ a)).
+    { r_wf WF0. }
+    i. guclo hframeC_aux_spec. econs.
+    { instantiate (1:=a). eapply URA.wf_mon. instantiate (1:=b). r_wf WF0. }
+    guclo hmonoC_spec. econs.
+    { eapply H. }
+    i. iIntros "H0". iModIntro. iIntros "H1".
+    iPoseProof (H0 with "H1") as "H1".
+    iMod "H1". iApply "H1". iApply "H0".
+  Qed.
+
+  Lemma back_upd R_src R_tgt
+        (Q: Any.t -> Any.t -> R_src -> R_tgt -> iProp)
+        r g fuel f_src f_tgt st_src itr_src st_tgt itr_tgt
+    :
+      bi_entails
+        (#=> (back r g Q fuel f_src f_tgt (st_src, itr_src) (st_tgt, itr_tgt)))
+        (back r g Q fuel f_src f_tgt (st_src, itr_src) (st_tgt, itr_tgt)).
+  Proof.
+    red. unfold Entails. autorewrite with iprop.
+    unfold back in *. i.
+    red in H. unfold bi_bupd_bupd in H. ss. unfold Upd in H. autorewrite with iprop in H.
+    hexploit H; eauto. i. des.
+    hexploit H1; eauto.
+  Qed.
+
+  Lemma back_bind R_src R_tgt S_src S_tgt
+        (Q: Any.t -> Any.t -> R_src -> R_tgt -> iProp)
+        r g fuel f_src f_tgt st_src (itr_src: itree hEs S_src)
+        ktr_src st_tgt (itr_tgt: itree Es S_tgt) ktr_tgt
+    :
+      bi_entails
+        (back r g (fun st_src st_tgt ret_src ret_tgt => back r g Q None false false (st_src, ktr_src ret_src) (st_tgt, ktr_tgt ret_tgt)) fuel f_src f_tgt (st_src, itr_src) (st_tgt, itr_tgt))
+        (back r g Q fuel f_src f_tgt (st_src, itr_src >>= ktr_src) (st_tgt, itr_tgt >>= ktr_tgt)).
+  Proof.
+    red. unfold Entails. autorewrite with iprop.
+    unfold back in *. i.
+    guclo hbindC_spec. econs.
+    { eapply H; eauto. }
+    i. inv POST. eapply IPROP. eauto.
+  Qed.
+
+  Lemma back_call_impure
+        (Q: Any.t -> Any.t -> Any.t -> Any.t -> iProp)
+        r g fuel f_src f_tgt st_src st_tgt fn arg_src arg_tgt
+        fsp x w0
+        (SPEC: stb fn = Some fsp)
+        (MEASURE: o = ord_top)
+        (NPURE: fsp.(measure) x = ord_top)
+    :
+      bi_entails
+        ((#=> ((fsp.(precond) (Some mn) x arg_src arg_tgt: iProp) ** I w0 st_src st_tgt))
+           **
+           (∀ st_src st_tgt ret_src ret_tgt,
+               ((∃ w1, I w1 st_src st_tgt ** ⌜le w0 w1⌝) ** (fsp.(postcond) (Some mn) x ret_src ret_tgt: iProp)) -* #=> Q st_src st_tgt ret_src ret_tgt))
+        (back r g Q fuel f_src f_tgt (st_src, trigger (Call fn arg_src)) (st_tgt, trigger (Call fn arg_tgt))).
+  Proof.
+    red. unfold Entails. autorewrite with iprop.
+    unfold back in *. i.
+    match (type of H) with
+    | ?P _ =>
+      assert (CUR: current_iProp ctx P)
+    end.
+    { econs; eauto. }
+    apply current_iPropL_convert in CUR.
+    mDesAll. mUpd "H". mDesSep "H".
+    ired_both. gstep. econs; eauto.
+    { eapply current_iProp_entail; [eapply CUR|]. start_ipm_proof.
+      iSplitR "H"; [|iExact "H"].
+      iSplitR "A1"; [|iExact "A1"].
+      iExact "A".
+    }
+    i. apply current_iPropL_convert in ACC.
+    mDesAll. mSpcUniv "H" with st_src1.
+    mSpcUniv "H" with st_tgt1.
+    mSpcUniv "H" with ret_src.
+    mSpcUniv "H" with ret_tgt.
+    mAssert (#=> Q st_src1 st_tgt1 ret_src ret_tgt) with "*".
+    { iApply "H". iSplitR "A"; [|iExact "A"].
+      iExists w1. iSplit; ss.
+    }
+    mUpd "A2".
+    gstep. econs.
+    eapply current_iProp_entail; [eapply ACC|].
+    start_ipm_proof. auto.
   Qed.
 End SIM.
