examples/multwhile/MultWhile01proof.v
@@ -55,118 +55,118 @@ Section SIMMODSEM.
   (* trivial invariant *)
   Let Inv := (fun (_: unit) (_ _: Any.t) => (True: iProp)%I).
 
-  Definition to_irel (R_src R_tgt: Type)
-             (RR: R_src -> R_tgt -> Any.t -> Any.t -> iProp)
-             (st_src: Any.t) (st_tgt: Any.t)
-             (r_src: R_src) (r_tgt: R_tgt): Prop :=
-    exists mr_src mp_src,
-      (<<SRC: st_src = Any.pair mp_src (Any.upcast mr_src)>>) /\
-      (<<IPROP: RR r_src r_tgt mp_src st_tgt mr_src>>).
+(*   Definition to_irel (R_src R_tgt: Type) *)
+(*              (RR: R_src -> R_tgt -> Any.t -> Any.t -> iProp) *)
+(*              (st_src: Any.t) (st_tgt: Any.t) *)
+(*              (r_src: R_src) (r_tgt: R_tgt): Prop := *)
+(*     exists mr_src mp_src, *)
+(*       (<<SRC: st_src = Any.pair mp_src (Any.upcast mr_src)>>) /\ *)
+(*       (<<IPROP: RR r_src r_tgt mp_src st_tgt mr_src>>). *)
 
-  Theorem correct: refines2 [MultWhile0.Mul] [MultWhile1.Mul].
-  Proof.
-    (* boring part *)
-    eapply adequacy_local2. econs; ss.
-    i. econstructor 1 with (wf:=mk_wf Inv) (le:=top2); et.
-    { ss. }
-    2: { exists tt. unfold Inv. econs; ss; red; uipropall. }
-    econs; ss. unfold mulF, ccallU. init. harg.
-    mDesAll. des_ifs. gfinal. right.    
-    hexploit (@hsim_adequacy_aux _ unit top2 Inv "Mul" (STB.to_stb Mulstb) (ord_pure n) true false (mp_src) mp_tgt).
-    2:{ i. instantiate (8:=None) in H.
-        instantiate (4:=ctx) in H.
-        instantiate (4:=(z, z0)) in H.
-        instantiate (4:=mn) in H.
-        instantiate (4:=Any.upcast mr_src) in H.
-        instantiate (4:=w) in H.
-        instantiate (1:=    ` varg0 : Z * Z <- unwrapU (Any.downcast varg);;
-                                      ` vret : Z <-
-                                               (let
-                                                   '(a, b) := varg0 in
-                                                 ITree.iter (λ '(a0, res), if (0 <? a0)%Z then Ret (inl ((a0 - 1)%Z, (res + b)%Z)) else Ret (inr res)) (a, 0%Z));;
-                                               Ret (Any.upcast vret)) in H.
-        ss.
-        match goal with
-        | H: ?P0 |- ?P1 => replace P1 with P0
-        end.
-        { eapply H. }
-        f_equal. f_equal. ss. f_equal. f_equal.
+(*   Theorem correct: refines2 [MultWhile0.Mul] [MultWhile1.Mul]. *)
+(*   Proof. *)
+(*     (* boring part *) *)
+(*     eapply adequacy_local2. econs; ss. *)
+(*     i. econstructor 1 with (wf:=mk_wf Inv) (le:=top2); et. *)
+(*     { ss. } *)
+(*     2: { exists tt. unfold Inv. econs; ss; red; uipropall. } *)
+(*     econs; ss. unfold mulF, ccallU. init. harg. *)
+(*     mDesAll. des_ifs. gfinal. right.     *)
+(*     hexploit (@hsim_adequacy_aux _ unit top2 Inv "Mul" (STB.to_stb Mulstb) (ord_pure n) true false (mp_src) mp_tgt). *)
+(*     2:{ i. instantiate (8:=None) in H. *)
+(*         instantiate (4:=ctx) in H. *)
+(*         instantiate (4:=(z, z0)) in H. *)
+(*         instantiate (4:=mn) in H. *)
+(*         instantiate (4:=Any.upcast mr_src) in H. *)
+(*         instantiate (4:=w) in H. *)
+(*         instantiate (1:=    ` varg0 : Z * Z <- unwrapU (Any.downcast varg);; *)
+(*                                       ` vret : Z <- *)
+(*                                                (let *)
+(*                                                    '(a, b) := varg0 in *)
+(*                                                  ITree.iter (λ '(a0, res), if (0 <? a0)%Z then Ret (inl ((a0 - 1)%Z, (res + b)%Z)) else Ret (inr res)) (a, 0%Z));; *)
+(*                                                Ret (Any.upcast vret)) in H. *)
+(*         ss. *)
+(*         match goal with *)
+(*         | H: ?P0 |- ?P1 => replace P1 with P0 *)
+(*         end. *)
+(*         { eapply H. } *)
+(*         f_equal. f_equal. ss. f_equal. f_equal. *)
 
-        instantiate (6:=ctx).
-
-
-
-        instantiate (1:=(APC;; trigger (Choose Any.t))) in H.
-
-        ss.
+(*         instantiate (6:=ctx). *)
 
 
-        eapply H. mDesAll. des; clarify.
+
+(*         instantiate (1:=(APC;; trigger (Choose Any.t))) in H. *)
+
+(*         ss. *)
 
 
-        instantiate (4:=w) in H.
-        instantiate (8:=None) in H.
-        instantiate (7:=None) in H.
-
- ss.
-        instantiate (2:=x) in H.
+(*         eapply H. mDesAll. des; clarify. *)
 
 
-hsim_adequacy_aux
-     : ∀ (world : Type) (le : relation world) (I : world → Any.t → Any.t → iProp) (mn : string) (stb : string → option fspec) 
-         (o : ord) (f_src f_tgt : bool) (st_src st_tgt : Any.t) (itr_src : itree (hAPCE +' Es) Any.t) (itr_tgt : itree Es Any.t) 
-         (mr_src : Any.t) (ctx : Σ) (X : Type) (x : X) (Q : option string → X → Any.t → Any.t → iProp) (mn_caller : option string) 
-         (fuel : option Ord.t) (w0 : world),
-         hsim I mn stb o (st_tgt, itr_tgt)
-         → paco8 (_sim_itree (mk_wf I) le) bot8 Any.t Any.t (lift_rel (mk_wf I) le w0 eq) f_src f_tgt w0
-             (Any.pair st_src mr_src, mylift mn stb o fuel mn_caller x ctx Q itr_src) (st_tgt, itr_tgt)
+(*         instantiate (4:=w) in H. *)
+(*         instantiate (8:=None) in H. *)
+(*         instantiate (7:=None) in H. *)
+
+(*  ss. *)
+(*         instantiate (2:=x) in H. *)
 
 
-        match goal with
-        | H: ?P0 |- ?P1 => replace P1 with P0
-        end.
-        { eapply H. }
-        instantiate (6:=ctx).
-
-        eapply f_equal.
-
-        f_equal.
-        
-eapply f_equal.
-        repeat f_equal.
+(* hsim_adequacy_aux *)
+(*      : ∀ (world : Type) (le : relation world) (I : world → Any.t → Any.t → iProp) (mn : string) (stb : string → option fspec)  *)
+(*          (o : ord) (f_src f_tgt : bool) (st_src st_tgt : Any.t) (itr_src : itree (hAPCE +' Es) Any.t) (itr_tgt : itree Es Any.t)  *)
+(*          (mr_src : Any.t) (ctx : Σ) (X : Type) (x : X) (Q : option string → X → Any.t → Any.t → iProp) (mn_caller : option string)  *)
+(*          (fuel : option Ord.t) (w0 : world), *)
+(*          hsim I mn stb o (st_tgt, itr_tgt) *)
+(*          → paco8 (_sim_itree (mk_wf I) le) bot8 Any.t Any.t (lift_rel (mk_wf I) le w0 eq) f_src f_tgt w0 *)
+(*              (Any.pair st_src mr_src, mylift mn stb o fuel mn_caller x ctx Q itr_src) (st_tgt, itr_tgt) *)
 
 
-        2:{ 
+(*         match goal with *)
+(*         | H: ?P0 |- ?P1 => replace P1 with P0 *)
+(*         end. *)
+(*         { eapply H. } *)
+(*         instantiate (6:=ctx). *)
 
-eapply H.
+(*         eapply f_equal. *)
 
-hsim_adequacy_aux
-     : ∀ (world : Type) (le : relation world) (I : world → Any.t → Any.t → iProp) (mn : string) (stb : string → option fspec) 
-         (o : ord) (f_src f_tgt : bool) (st_src st_tgt : Any.t) (itr_src : itree (hAPCE +' Es) Any.t) (itr_tgt : itree Es Any.t) 
-         (mr_src : Any.t) (ctx : Σ) (X : Type) (x : X) (Q : option string → X → Any.t → Any.t → iProp) (mn_caller : option string) 
-         (fuel : option Ord.t) (w0 : world),
-         hsim I mn stb o (st_tgt, itr_tgt)
-         → paco8 (_sim_itree (mk_wf I) le) bot8 Any.t Any.t (lift_rel (mk_wf I) le w0 eq) f_src f_tgt w0
-             (Any.pair st_src mr_src, mylift mn stb o fuel mn_caller x ctx Q itr_src) (st_tgt, itr_tgt)
+(*         f_equal. *)
+
+(* eapply f_equal. *)
+(*         repeat f_equal. *)
 
 
-    destruct x as [a b]. mDesAll. des; clarify. simpl. steps. astop. simpl. steps.
-    (* bind *)
-    guclo lbindC_spec. eapply lbindR_intro with (RR := fun st_src _ r_src r_tgt => r_src = r_tgt↑ /\ r_tgt = (a * b)%Z /\ st_src = Any.pair mp_src (Any.upcast mr_src)).
-    { steps. instantiate (1:=tt).
-      (* induction on a *)
-      assert (exists n, <<EQ: a = Z.of_nat n>> /\ <<SUM: (a * b + 0 = a * b)%Z>>).
-      { exists (Z.to_nat a). rewrite Z2Nat.id; auto. splits; auto. lia. }
-      des. deflag. revert EQ SUM. generalize a at 1 2 5. generalize 0%Z at 1 3. induction n; i.
-      (* a = 0 *)
-      { rewrite unfold_iter. subst. ss. steps. force_l. eexists. steps. }
-      (* a = S _ *)
-      { rewrite unfold_iter. subst. ss. steps. deflag. eapply IHn.
-        { lia. }
-        { lia. }
-      }
-    }
-    { i. des. clarify. steps. hret tt; auto. }
-  Qed.
+(*         2:{  *)
+
+(* eapply H. *)
+
+(* hsim_adequacy_aux *)
+(*      : ∀ (world : Type) (le : relation world) (I : world → Any.t → Any.t → iProp) (mn : string) (stb : string → option fspec)  *)
+(*          (o : ord) (f_src f_tgt : bool) (st_src st_tgt : Any.t) (itr_src : itree (hAPCE +' Es) Any.t) (itr_tgt : itree Es Any.t)  *)
+(*          (mr_src : Any.t) (ctx : Σ) (X : Type) (x : X) (Q : option string → X → Any.t → Any.t → iProp) (mn_caller : option string)  *)
+(*          (fuel : option Ord.t) (w0 : world), *)
+(*          hsim I mn stb o (st_tgt, itr_tgt) *)
+(*          → paco8 (_sim_itree (mk_wf I) le) bot8 Any.t Any.t (lift_rel (mk_wf I) le w0 eq) f_src f_tgt w0 *)
+(*              (Any.pair st_src mr_src, mylift mn stb o fuel mn_caller x ctx Q itr_src) (st_tgt, itr_tgt) *)
+
+
+(*     destruct x as [a b]. mDesAll. des; clarify. simpl. steps. astop. simpl. steps. *)
+(*     (* bind *) *)
+(*     guclo lbindC_spec. eapply lbindR_intro with (RR := fun st_src _ r_src r_tgt => r_src = r_tgt↑ /\ r_tgt = (a * b)%Z /\ st_src = Any.pair mp_src (Any.upcast mr_src)). *)
+(*     { steps. instantiate (1:=tt). *)
+(*       (* induction on a *) *)
+(*       assert (exists n, <<EQ: a = Z.of_nat n>> /\ <<SUM: (a * b + 0 = a * b)%Z>>). *)
+(*       { exists (Z.to_nat a). rewrite Z2Nat.id; auto. splits; auto. lia. } *)
+(*       des. deflag. revert EQ SUM. generalize a at 1 2 5. generalize 0%Z at 1 3. induction n; i. *)
+(*       (* a = 0 *) *)
+(*       { rewrite unfold_iter. subst. ss. steps. force_l. eexists. steps. } *)
+(*       (* a = S _ *) *)
+(*       { rewrite unfold_iter. subst. ss. steps. deflag. eapply IHn. *)
+(*         { lia. } *)
+(*         { lia. } *)
+(*       } *)
+(*     } *)
+(*     { i. des. clarify. steps. hret tt; auto. } *)
+(*   Qed. *)
 
 End SIMMODSEM.
